Tactic.v
@@ -142,8 +142,7 @@ end.
 Ltac mor2 := intros; mor2'; try reflexivity.
 Ltac test2 := intros; mor2'.
 
-
-Theorem wut2 :
+Goal
   forall (C : Cat) (X Y Z W V T: Ob C) (f f' : Hom X Y) (g : Hom Y Z)
     (h : Hom Z W) (i : Hom W V) (j : Hom V T), f == f' ->
       ((f .> (g .> h)) .> i) .> j == f' .> g .> h .> i .> j.
@@ -151,7 +150,7 @@ Proof.
   test2. reflexivity.
 Qed.
 
-Theorem wut3 :
+Goal
   forall (C : Cat) (X Y Z W V T: Ob C) (f f' : Hom X Y) (g g' : Hom Y Z)
     (h : Hom Z W) (i : Hom W V) (j : Hom V T), f .> g == f' .> g' ->
       ((f .> (g .> h)) .> i) .> j == f' .> (g' .> h) .> i .> j.
@@ -159,67 +158,10 @@ Proof.
   test2.
 Abort.
 
-Theorem wut4 :
+Goal
   forall (C : Cat) (X Y Z W V T: Ob C) (f f' : Hom X Y) (g g' : Hom Y Z)
     (h : Hom Z W) (i : Hom W V) (j : Hom V T),
       f == f .> id _ .> id _.
 Proof.
   test. reflexivity.
 Abort.
-
-Fixpoint simplify {C : Cat} {X Y : Ob C} (e : exp X Y) : exp X Y :=
-match e with
-    | Id X => Id X
-    | Var f => Var f
-    | Comp e1 e2 => Comp (simplify e1) (simplify e2)
-end.
-
-Fixpoint simplify' {C : Cat} {X Y : Ob C} (e : exp X Y) {struct e} : exp X Y.
-Proof.
-  destruct e.
-    exact (Id X).
-    exact (Var h).
-    destruct (simplify' _ _ _ e1); clear e1.
-      exact (simplify' _ _ _ e2).
-      exact (Comp (Var h) (simplify' _ _ _ e2)).
-      exact (Comp (Comp e3 e4) (simplify' _ _ _ e2)).
-Defined.
-
-Theorem simplify_correct :
-  forall (C : Cat) (X Y : Ob C) (e : exp X Y),
-    expDenote (simplify e) == expDenote e.
-Proof.
-  induction e; simpl; try rewrite IHe1, IHe2; reflexivity.
-Qed.
-
-Theorem simplify'_correct :
-  forall (C : Cat) (X Y : Ob C) (e : exp X Y),
-    expDenote (simplify' e) == expDenote e.
-Proof.
-  induction e; simpl; try reflexivity.
-    destruct (simplify' e1); simpl in *;
-    try rewrite <- IHe1; try rewrite IHe2; cat.
-Qed.
-
-Print simplify'.
-
-Fixpoint simplify2 {C : Cat} {X Y : Ob C} (e : exp X Y) : exp X Y :=
-match e in (exp o o0) return (exp o o0) with
-  | Id A => Id A
-  | Var f => Var f
-  | @Comp _ A B C e1 e2 =>
-      match simplify2 e1 in (exp A B) with
-      (*return exp A B -> exp B C -> exp A C with*)
-          | Id A => fun (_ : exp A A) (e2 : exp A C) => simplify2 e2
-          | e1' => fun _ e2 => Comp e1' (simplify2 e2)
-      end e1 e2
-end.
-
-Theorem simplify2_correct :
-  forall (C : Cat) (X Y : Ob C) (e : exp X Y),
-    expDenote (simplify2 e) == expDenote e.
-Proof.
-  induction e; simpl; try reflexivity.
-    destruct (simplify2 e1); simpl in *;
-    try rewrite <- IHe1; try rewrite IHe2; cat.
-Qed.
