Tactic2.v
@@ -1,0 +1,217 @@
+Add Rec LoadPath "/home/zeimer/Code/Coq".
+
+Require Import Cat.
+
+Inductive exp {C : Cat} : Ob C -> Ob C -> Type :=
+    | Id : forall X : Ob C, exp X X
+    | Var : forall X Y : Ob C, Hom X Y -> exp X Y
+    | Comp : forall X Y Z : Ob C,
+        exp X Y -> exp Y Z -> exp X Z.
+
+Arguments Id [C] _.
+Arguments Var [C X Y] _.
+Arguments Comp [C X Y Z] _ _.
+
+Fixpoint expDenote {C : Cat} {X Y : Ob C} (e : exp X Y)
+    : Hom X Y :=
+match e with
+    | Id X => id X
+    | Var f => f
+    | Comp e1 e2 => expDenote e1 .> expDenote e2
+end.
+
+Fixpoint simplify {C : Cat} {X Y : Ob C} (e : exp X Y) {struct e} : exp X Y.
+Proof.
+  destruct e.
+    exact (Id _).
+    exact (Var h).
+    Hint Constructors exp. destruct (simplify _ _ _ e1) as [| ? ? f1 | ? ? ? e11 e12]; clear e1.
+      exact (simplify _ _ _ e2).
+      destruct (simplify _ _ _ e2) as [| ? ? f2 | ? ? ? e21 e22]; clear e2.
+        exact (Var f1).
+        exact (Comp (Var f1) (Var f2)).
+        exact (Comp (Var f1) (Comp e21 e22)).
+      destruct (simplify _ _ _ e2) as [| ? ? f2 | ? ? ? e21 e22]; clear e2.
+        exact (Comp e11 e12).
+        exact (Comp (Comp e11 e12) (Var f2)).
+        exact (Comp (Comp e11 e12) (Comp e21 e22)).
+Defined.
+
+Print simplify.
+
+Theorem simplify_correct :
+  forall (C : Cat) (X Y : Ob C) (e : exp X Y),
+    expDenote (simplify e) == expDenote e.
+Proof.
+  induction e; simpl; try reflexivity.
+    destruct (simplify e1); destruct (simplify e2); simpl in *;
+    try rewrite <- IHe1; try rewrite <- IHe2; cat.
+Qed.
+
+Inductive HomList {C : Cat} : Ob C -> Ob C -> Type :=
+    | HomNil : forall X : Ob C, HomList X X
+    | HomCons : forall X Y Z : Ob C,
+        Hom X Y -> HomList Y Z -> HomList X Z.
+
+Arguments HomNil [C] _.
+Arguments HomCons [C X Y Z] _ _.
+
+Fixpoint expDenoteHL {C : Cat} {X Y : Ob C} (l : HomList X Y)
+    : Hom X Y :=
+match l with
+    | HomNil X => id X
+    | HomCons h t => h .> expDenoteHL t
+end.
+
+Fixpoint Happ {C : Cat} {X Y Z : Ob C} (l1 : HomList X Y)
+    : HomList Y Z -> HomList X Z :=
+match l1 with
+    | HomNil _ => fun l2 => l2
+    | HomCons h t => fun l2 => HomCons h (Happ t l2)
+end.
+
+Infix "+++" := (Happ) (at level 40).
+
+Fixpoint flatten {C : Cat} {X Y : Ob C} (e : exp X Y)
+    : HomList X Y :=
+match e with
+    | Id X => HomNil X
+    | Var f => HomCons f (HomNil _)
+    | Comp e1 e2 => flatten e1 +++ flatten e2
+end.
+
+Lemma expDenoteHL_comp_app :
+  forall (C : Cat) (X Y Z : Ob C) (l1 : HomList X Y) (l2 : HomList Y Z),
+    expDenoteHL l1 .> expDenoteHL l2 == expDenoteHL (l1 +++ l2).
+Proof.
+  induction l1; simpl; intros.
+    rewrite id_left. reflexivity.
+    assocr. rewrite IHl1. reflexivity.
+Qed.
+
+Theorem flatten_correct :
+  forall (C : Cat) (X Y : Ob C) (e : exp X Y),
+    expDenoteHL (flatten e) == expDenote e.
+Proof.
+  induction e; cat.
+    rewrite <- expDenoteHL_comp_app. apply comp_Proper; auto.
+Qed.
+
+Theorem cat_reflect :
+  forall (C : Cat) (X Y : Ob C) (e1 e2 : exp X Y),
+    expDenoteHL (flatten (simplify e1)) ==
+    expDenoteHL (flatten (simplify e2)) ->
+      expDenote e1 == expDenote e2.
+Proof.
+  intros.
+  do 2 rewrite flatten_correct in H.
+  do 2 rewrite simplify_correct in H.
+  assumption.
+Qed.
+
+Ltac reify mor :=
+match mor with
+    | id ?X => constr:(Id X)
+    | ?f .> ?g =>
+        let e1 := reify f in
+        let e2 := reify g in constr:(Comp e1 e2)
+    | ?f => match type of f with
+        | Hom ?X ?Y => constr:(Var f)
+        | _ => fail
+    end
+end.
+
+Ltac mor' := intros;
+match goal with
+    | |- ?f == ?g =>
+        let e1 := reify f in
+        let e2 := reify g in
+          change (expDenote e1 == expDenote e2);
+          apply cat_reflect; simpl
+end.
+
+Ltac mor := mor'; reflexivity.
+
+Ltac wut := repeat apply comp_Proper; cat.
+Ltac wuut := mor'; wut.
+
+Goal forall (C : Cat) (X Y Z W V T: Ob C) (f : Hom X Y) (g : Hom Y Z)
+    (h : Hom Z W) (i : Hom W V) (j : Hom V T),
+      ((f .> (g .> h)) .> i) .> j == f .> g .> h .> i .> j.
+Proof.
+  mor'. reflexivity.
+Qed.
+
+Goal
+  forall (C : Cat) (X Y Z W V T: Ob C) (f f' : Hom X Y) (g : Hom Y Z)
+    (h : Hom Z W) (i : Hom W V) (j : Hom V T), f == f' ->
+      ((f .> (g .> h)) .> i) .> j == f' .> g .> h .> i .> j.
+Proof.
+  mor'.
+Restart.
+  wuut.
+Qed.
+
+Goal
+  forall (C : Cat) (X Y Z W V T: Ob C) (f f' : Hom X Y) (g g' : Hom Y Z)
+    (h : Hom Z W) (i : Hom W V) (j : Hom V T), f .> g == f' .> g' ->
+      ((f .> (g .> h)) .> i) .> j == f' .> (g' .> h) .> i .> j.
+Proof.
+  mor'.
+Restart.
+  wuut.
+Abort.
+
+Goal
+  forall (C : Cat) (X Y Z W V T: Ob C) (f f' : Hom X Y) (g g' : Hom Y Z)
+    (h : Hom Z W) (i : Hom W V) (j : Hom V T),
+      f == f .> id _ .> id _.
+Proof.
+  mor'. reflexivity.
+Qed.
+
+Fixpoint simplify' {C : Cat} {X Y : Ob C} (e : exp X Y) {struct e} : exp X Y :=
+match e in (exp o o0) return (exp o o0) with
+  | Id X0 => Id X0
+  | Var h => Var h
+  | @Comp _ X0 Y0 Z e1 e2 =>
+    match simplify' e1 in (exp o o0)
+    return (exp o o0 -> exp o0 Z -> exp o Z) with
+      | Id X1 =>
+          fun _ (e2 : exp X1 Z) => simplify' e2
+      | @Var _ X1 Y1 f1 =>
+          fun _ (e2 : exp Y1 Z) =>
+          match simplify' e2 in (exp o o0)
+          return (exp o o0 -> Hom X1 o -> exp X1 o0)
+          with
+          | Id X2 => fun _ (f1 : Hom X1 X2) => Var f1
+          | @Var _ X2 Y2 f2 =>
+              fun _ (f1 : Hom X1 X2) => Comp (Var f1) (Var f2)
+          | @Comp _ X2 Y2 Z0 e21 e22 =>
+              fun _ (f2 : Hom X1 X2) =>
+              Comp (Var f2) (Comp e21 e22)
+          end e2 f1
+      | @Comp _ X1 Y1 Z0 e11 e12 =>
+          fun _ (e2 : exp Z0 Z) =>
+          match simplify' e2 in (exp o o0)
+          return (exp o o0 -> exp Y1 o -> exp X1 o0)
+          with
+          | Id X2 => fun _ (e12 : exp Y1 X2) => Comp e11 e12
+          | @Var _ X2 Y2 f2 =>
+              fun _ (e12 : exp Y1 X2) =>
+              Comp (Comp e11 e12) (Var f2)
+          | @Comp _ X2 Y2 Z1 e21 e22 =>
+              fun _ (e12 : exp Y1 X2) =>
+              Comp (Comp e11 e12) (Comp e21 e22)
+          end e2 e12
+      end e1 e2
+end.
+
+Theorem simplify'_correct :
+  forall (C : Cat) (X Y : Ob C) (e : exp X Y),
+    expDenote (simplify' e) == expDenote e.
+Proof.
+  induction e; simpl; try reflexivity.
+    destruct (simplify' e1); destruct (simplify' e2); simpl in *;
+    try rewrite <- IHe1; try rewrite <- IHe2; cat.
+Qed.
